

2.1.2

Mehmet Ali Kırnızlıoğlu
19253055

a-) $a(ba)^*$

b-) a^*b

c-) aynı sayıda a's ve b's'e sahip olan ve hiçbir öneki a's'den 2 veya daha fazla b's içermeyen tüm dizeler

d-) aynı sayıda a's ve b's'e sahip olan ve hiçbir önekin birden fazla a's'ya sahip olmadığı tüm dizeler veya tersi

e-) aab veya bba alt dizelerini içeren tüm dizeler

2.1.3

a-) $\{w: \text{each } a \text{ in } w \text{ immediately preceded by } ab\}$:

$K = \{q_0, q_1, q_2\}$

$\Sigma = \{a, b\}$

$\delta = q_0$

$F = \{q_0, q_1\}$

q	σ	$\delta(q, \sigma)$
q_0	a	q_1
q_0	b	q_1
q_1	a	q_0
q_1	b	q_2
q_2	a	q_1
q_2	b	q_2

b-) $\{w: \text{neither } abab \text{ is a substring of } w\}$:

$K = \{q_0, q_1, q_2, q_3, q_4\}$

$\Sigma = \{a, b\}$

$\delta = q_0$

$F = \{q_4\}$

q	σ	$\delta(q, \sigma)$
q_0	a	q_1
q_0	b	q_0
q_1	a	q_1
q_1	b	q_2
q_2	a	q_3
q_2	b	q_0
q_3	a	q_1
q_3	b	q_4
q_4	a	q_4
q_4	b	q_4

c-) $\{w: \text{neither } aa \text{ nor } bb \text{ is a substring of } w\}$:

$K = \{q_0, q_1, q_2, q_3\}$

$\Sigma = \{a, b\}$

$\delta = q_0$

$F = \{q_0, q_1, q_2\}$

q	σ	$\delta(q, \sigma)$
q_0	a	q_1
q_0	b	q_2
q_1	a	q_3
q_1	b	q_2
q_2	a	q_1
q_2	b	q_3
q_3	a	q_3
q_3	b	q_3

d-) $\{w: w \text{ has an odd number of a's and even number of b's}\}$

$L = \{q_0, q_1, q_2, q_3\}$

$\Sigma = \{a, b\}$

$\delta = q_0$

$F = \{q_1\}$

q	σ	$\delta(q, \sigma)$
q_0	a	q_1
q_0	b	q_2
q_1	a	q_0
q_1	b	q_3
q_2	a	q_3
q_2	b	q_0
q_3	a	q_2
q_3	b	q_1

e-) $\{w: w \text{ has both ab and ba as substrings}\}$

$L = \{q_0, q_1, q_2, q_3, q_4, q_5\}$

$\Sigma = \{a, b\}$

$\delta = q_0$

$F = \{q_5\}$

q	σ	$\delta(q, \sigma)$
q_0	a	q_1
q_0	b	q_1
q_1	a	q_2
q_1	b	q_1
q_2	a	q_3
q_2	b	q_4
q_3	a	q_2
q_3	b	q_5
q_4	a	q_5
q_4	b	q_5
q_5	a	q_5
q_5	b	q_5

2.1.4

Let M' be the machine formed from M by deleting the unreachable state p . We show $L(M) = L(M')$. As a lemma, we will show that $(q_1, \pi_1) \vdash^* M (q_2, \pi_2)$ implies $(q_1, x, y) \vdash^* M' (q_2, y)$, where q_1 is any reachable state of M (q_1 is trivially reachable, as well, given the hypothesis) we prove this lemma by induction on $|w|$.

Basic step $|x| = 0$ then $x = \epsilon$, so that $(q_1, y) \vdash^* M (q_2, y)$ which forces $q_1 = q_2$. Thus by reflexivity $(q_1, y) \vdash^* M' (q_2, y)$.

Induction step: suppose $(q_1, x, y) \vdash^* M (q_2, y)$ where $|x| = n+1$. Then $x = w\sigma$, where $\sigma \in \Sigma$ and $|w| = n$. let r be the state such that $(q_1, x\sigma) \vdash^* M (r, y)$. Because q_1 is reachable there is some string σ such that $(s, \sigma) \vdash^* M (q_1, \epsilon)$. Therefore $(s, \sigma) \vdash^* M$ are both states of M' and $\delta_{M'}$, whenever it exists is the same as δ_M , $\delta_{M'}(r, \sigma) = \delta_M(r, \sigma) = q_2$, so that $(r, y) \vdash^* M' (q_2, y)$ and thus $(q_1, y) \vdash^* M' (q_2, y)$.

Suppose now, that $w \in L(M)$. By definition of $L(M)$, $(s, w) \vdash^* M (q, \epsilon)$ where $q \in F$. By the lemma $(s, w) \vdash^* M' (q, \epsilon)$ so that $w \in L(M')$.